\documentclass[12pt]{article}
\usepackage{mathtools}
\usepackage{amsthm}
\usepackage{amsfonts}
\usepackage{amssymb}
\usepackage{fontspec}
\usepackage{xfrac}
\usepackage{array}
\usepackage{siunitx}
\usepackage{gensymb}
\usepackage{enumitem}
\usepackage{dirtytalk}
\usepackage{bm}
\title{Fields}
\author{Zoë Sparks}

\begin{document}

\theoremstyle{definition}

\sisetup{quotient-mode=fraction}
\newtheorem{thm}{Theorem}
\newtheorem*{nthm}{Theorem}
\newtheorem{sthm}{}[thm]
\newtheorem{lemma}{Lemma}[thm]
\newtheorem*{cor}{Corollary}
\newtheorem*{prop}{Property}
\newtheorem*{defn}{Definition}
\newtheorem*{comm}{Comment}
\newtheorem*{exm}{Example}

\maketitle

\begin{defn}
  A \textbf{field} $F$ is a set of objects $x, y, z, …$ together
  with two operations on the elements of $F$: \textbf{addition},
  which associates each pair of elements $x, y$ in $F$ with an
  element $x + y$ in $F$, and \textbf{multiplication}, which
  associates each pair of elements $x, y$ with an element $xy$ in
  $F$. Furthermore, these two operations should satisfy the
  following conditions:

  \begin{enumerate}
      \item Addition is commutative: $x + y = y + x$ for all $x,
        y$ in $F$.
      \item Addition is associative: $x + (y + z) = (x + y) + z$
        for all $x, y, z$ in $F$.
      \item There is a unique element $0$ (zero) in $F$ such that
        $x + 0 = x$ for every $x$ in $F$.
      \item For every $x$ in $F$ there is a unique element $-x$
        in $F$ such that $x + (-x) = 0$.
      \item Multiplication is commutative: $xy = yx$ for all $x,
        y$ in $F$.
      \item Multiplication is associative: $x(yz) = (xy)z$ for
        all $x, y, z$ in $F$.
      \item There is a unique element $1$ (one) in $F$ such that
        $1 \neq 0$ and $1x = x$ for every $x$ in $F$.
      \item For each element $x \neq 0$ in $F$ there is a unique
        element $x^{-1}$ (or $1/x$) in $F$ such that $xx^{-1} =
        1$.
      \item Multiplication distributes over addition: $x(y + z) =
        xy + xz$ for all $x, y, z$ in $F$.
  \end{enumerate}
\end{defn}

\begin{exm}
  The set of natural numbers $\mathbb{N}$ is not a field. $0$ is
  not a natural number, nor is $-n$ for any natural number $n$,
  nor $1/n$ (except in the case of $1$).
\end{exm}

\begin{exm}
  The set of integers $\mathbb{Z}$ is not a field. It comes
  close, but for an integer $n$, $1/n$ is not an integer unless
  $n = 1$ or $n = -1$.
\end{exm}

\begin{exm}
  The set of rational numbers $\mathbb{Q}$ is a field.
\end{exm}

\begin{exm}
  The set of real numbers $\mathbb{R}$ is a field.
\end{exm}

\begin{exm}
  The set of complex numbers $\mathbb{C}$ is a field.
\end{exm}

\begin{comm}
  In any field, one usually writes
  \begin{align*}
    x - y,\ \frac{x}{y},\ x + y + z,\ xyz,\ x^2,\ x^3,\ 2x,\ 3x,\ldots
  \end{align*}
  in place of
  \begin{align*}
    x + (-y),\ x \cdot \frac{1}{y},\ (x + y) + z,\ (xy)z,\ xx,\ xxx,\ x + x,\ x + x + x,\ldots
  \end{align*}
\end{comm}

\begin{thm} \label{thm:fieldaxforadd}
  The axioms for addition imply that
  \begin{enumerate}
    \item
      if $x + y = x + z$ then $y = z$,
    \item
      if $x + y = x$ then $y = 0$,
    \item
      if $x + y = 0 $ then $y = -x$, and
    \item
      $-(-x) = x$.
  \end{enumerate}

  \begin{proof}
    Let $F$ be a field such that $x,y \in F$. Let $a = x + y$ and $b = x + z$; then
    $a,b \in F$ and $a = b$, so $a-x,\ b-x \in F$ and $a - x = b - x$. Then $x + y -
    x = x + z - x$, so $x - x + y = x - x + z$, thus $0 + y = 0 + z$ and thus $y = z$.

    Letting $z = 0$ in (1) gives $x + y = x + 0$, which implies $y = 0$ by (1).
    Likewise, letting $z = -x$ in (1) gives $x + y = x - x = 0$, which implies $y =
    -x$ by (1). Last, letting $x = -x$ in (3) gives $y = -(-x)$, and if $-x - (-x) =
    0$, then $x - x - (-x) = x = -(-x)$.
  \end{proof}
\end{thm}

\begin{thm}
  The axioms for mulitplication imply that
  \begin{enumerate}
    \item
      if $x \neq 0$ and $xy = xz$, then $y = z$,
    \item
      if $x \neq 0$ and $xy = x$ then $y = 1$,
    \item
      if $x \neq 0$ and $xy = 1$ then $y = 1/x$, and
    \item
      if $x \neq 0$ then $1/(1/x) = x$.
  \end{enumerate}

  \begin{proof}
    Let $F$ be a field such that $x,y \in F$, and let $x \neq 0$. Let $a = xy$ and $b
    = xz$; then $a,b \in F$ and $a = b$, so $a/x,\ b/x \in F$ and $a/x = b/x$. Then
    $(xy)/x = (xz)/x$, so $y \cdot x/x = z \cdot x/x$, thus $y \cdot 1 = z \cdot 1$
    and thus $y = z$.

    Letting $z = 0$ in (1) gives $xy = x0$, which implies $y = 0$ by (1).  Likewise,
    letting $z = 1/x$ in (1) gives $xy = x(1/x) = 1$, which implies $y = 1/x$ by (1).
    Last, letting $x = 1/x$ in (3) gives $y = 1/(1/x)$, and if $1/x \cdot 1/(1/x) =
    1$, then $x \cdot 1/x \cdot 1/(1/x) = x \cdot 1 = 1 \cdot 1/(1/x) = 1/(1/x) = x$.
  \end{proof}
\end{thm}

\begin{thm}
  Let $F$ be a field. The field axioms imply that, for any $x,y \in F$,
  \begin{enumerate}
    \item
      $0x = 0$,
    \item
      if $x \neq 0$ and $y \neq 0$ then $xy \neq 0$,
    \item
      $(-x)y = -(xy) = x(-y)$, and
    \item
      $(-x)(-y) = xy$.
  \end{enumerate}

  \begin{proof}
    $0x = [x + (-x)]x = xx + (-xx) = 0$, which proves (1).

    If $x \neq 0$ and $y \neq 0$, there exist elements $1/x \in F$ and $1/y \in F$
    such that $x \cdot (1/x) = 1$ and $y \cdot (1/y) = 1$. Then $x(1/x)y(1/y) = 1(1)
    = 1 = xy(1/x)(1/y)$. By (1), $0 \cdot (1/x)(1/y) = 0$, and $1 \neq 0$, so $xy
    \neq 0$.

    $(-x)y + xy = y(-x) + yx = y(-x + x) = y0 = 0$. Therefore $(-x)y = -(xy)$.
    Likewise $x(-y) + xy = x(-y + y) = x0 = 0$, so $(-x)y = -(xy) = x(-y)$.

    If $(-x)y = -(xy)$, then $(-x)(-y) = -[x(-y)] = -[-(xy)] = xy$.
  \end{proof}
\end{thm}

\begin{defn}
  An \textbf{ordered field} is a field $F$ which is also an ordered set, with the
  order
  \begin{enumerate}
    \item
      $x + y < x + z$ if $x,y,z \in F$ and $y < z$, and
    \item
      $xy > 0$ if $x,y \in F$, $x > 0$, and $y > 0$.
  \end{enumerate}
  If $x > 0$, we say that $x$ is \textbf{positive}, and if $x < 0$, we say that $x$
  is \textbf{negative}.
\end{defn}

\begin{exm}
  $\mathbb{Q}$ is an ordered field.
\end{exm}

\begin{thm}
  The following is true in every ordered field:
  \begin{enumerate}
    \item
      if $x > 0$, then $-x < 0$ and vice versa,
    \item
      if $x > 0$ and $y < z$ then $xy < xz$,
    \item
      if $x < 0$ and $y < z$ then $xy > xz$,
    \item
      if $x \neq 0$ then $x^2 > 0$, and in particular $1 > 0$, and
    \item
      if $0 < x < y$, then $0 < 1/y < 1/x$.
  \end{enumerate}

  \begin{proof}
    If $x > 0$, then $-x + 0 < -x + x$, i.e. $-x < 0$. Likewise if $x < 0$, then $-x
    + x < -x + 0$, e.g. $0 < -x$. Also if $-x < 0$, then $x - x < x + 0$, i.e. $0 <
    x$, and if $0 < -x$, then $x + 0 < x - x$, i.e. $x < 0$.

    If $y < z$, then $z > y$, so $z - y > y - y = 0$. Then if $x > 0$, $x(z - y) >
    0$, so $xz - xy > 0$, e.g. $xz > xy$, so $xy < xz$. If $x < 0$, then $x(z - y) <
    0$, so $xz - xy < 0$, e.g. $xz < xy$, so $xy > xz$.

    Assume that $x > 0$. Then $xx = x^2 > 0$. Now assume that $x < 0$; then $xx = x^2
    > x0 = 0$.

    If $x > 0$, then if $v \leq 0$, $xv \leq 0$. However, $x(1/x) = 1 > 0$, so
    therefore $1/x > 0$. $1/y > 0$ by the same logic. Then if $0 < x < y$, $0 <
    x(1/x)(1/y) = 1/y < y(1/y)(1/x) = 1/x$.
  \end{proof}
\end{thm}

\begin{defn}
  A \textbf{subfield} of the field $F$ is a set $G \subseteq F$
  such that $G$ is a field under the same definitions of addition
  and mulitplication used with $F$.
\end{defn}

\begin{comm}
  If $G$ is a subfield of $F$, $0$ and $1$ are in $G$, and if $x,
  y$ are in $G$, then $(x + y)$, $xy$, $-x$, and $x^{-1}$ (if
  $x \neq 0$) are also in $G$.
\end{comm}

\begin{thm}
  \
  \begin{enumerate}
    \item
      If $x,y \in \mathbb{R}$ and $x > 0$, there is a positive integer $n$ such that
      $nx > y$. In other words, $\mathbb{R}$ is archimedean.
    \item
      If $x,y \in \mathbb{R}$ and $x < y$, there is a $p \in \mathbb{Q}$ such that $x
      < p < y$. In other words, $\mathbb{Q}$ is dense in $\mathbb{R}$.
  \end{enumerate}

  \begin{proof}
    \
    \begin{enumerate}
      \item
        Let $A = \{n \in \mathbb{Z}^+,\ x \in \mathbb{R}^+: nx\}$. Then $A \subset
        \mathbb{R}$ and $A$ is not empty (e.g. $1x = x \in A$). Assume (1) is false;
        then some $y \in \mathbb{R}$ is an upper bound of $A$. Because $\mathbb{R}$
        has the least-upper-bound property, there is then some $\alpha = \sup A \in
        \mathbb{R}$. Since $x > 0$, $\alpha - x < \alpha$, so $\alpha - x$ is not an
        upper bound of $A$. As such, $\alpha - x < mx$ for some $m \in \mathbb{Z}^+$.
        But then $\alpha - x + x = \alpha < mx + x = (m + 1)x = px$, where $p = m +
        1$ and thus $p > 0$. This implies that $\alpha$ is not an upper bound of $A$,
        which is contradictory, and thus (1) must be true.

      \item
        Since $x < y$, $y - x > 0$. As such, there is some positive integer $n$ such
        that $n(y - x) > 1$ by (1).  Also by (1), there are positive integers $m_1$
        and $m_2$ such that $m_1 > nx$ and $m_2 > -nx$; $nx$, $-nx$, and $1$ are real
        numbers and $m_1,m_2$ are positive, so $1m_1 > nx$ exists and so on. If $m_2
        > -nx$, then $-m_2 < nx$, so we then have $-m_2 < nx < m_1$.

        Consider an integer $m$ such that $-m_2 \leq m - 1 \leq nx < m \leq m_1$.
        Then $m \leq nx + 1$. Furthermore, if $n(y - x) > 1$, then $ny - nx > 1$, so
        $ny > nx + 1$. Therefore $nx < m \leq nx + 1 < ny$.

        Since $n > 0$ by definition, we then have $x < \frac{m}{n} \leq x +
        \frac{1}{n} < y$, i.e. $x < \frac{m}{n} < y$. Since $m$ and $n$ are integers,
        $\frac{m}{n} \in \mathbb{Q}$. We can thus say $p = \frac{m}{n}$; in full,
        this proves (2).
    \end{enumerate}
  \end{proof}
\end{thm}

\begin{thm} \label{thm:uniqrealroots}
  For every real $x > 0$ and every integer $n > 0$ there is one and only one positive
  real $y$ such that $y^n = x$. ($y$ is generally written as $\sqrt[n]{x}$ or
  $x^{1/n}$.)

  \begin{proof}
    Let $y_1,y_2 \in \mathbb{R}$ such that $0 < y_1 < y_2$; then $y_1^n < y_2^n$.
    This implies that if $y^n = x$ and $z^n = x$ for positive real numbers $y,z$,
    then $y = z$, i.e. there can only be one such $y$ at most.

    Let $E = \{t \in \mathbb{R}: 0 < t^n < x\}$. If $t = \frac{x}{1 + x}$, then $0
    < t < 1$, and then $0 < t^n \leq t < x$. Thus $t \in E$, so $E$ is not empty.

    If $t > 1 + x$, then $x < t \leq t^n$, and thus $t \notin E$. Therefore $1 + x$
    is an upper bound of $E$. By theorem \ref{thm:rlubsubq}, there is thus a positive
    real number $y = \sup E$.

    $y^n = x$. We will prove this by contradiction, showing that the inequalities
    $y^n < x$ and $y^n > x$ are both contradictory.

    Consider the identity $b^n - a^n = (b - a)(b^{n - 1} + b^{n - 2}a + \cdots +
    ba^{n - 2} + a^{n - 1})$. This implies that
    \begin{align*}
      b^n - a^n < (b - a)nb^{n-1}\ \ \text{when}\ 0 < a < b.
    \end{align*}

    Assume $y^x < x$. Let $h$ be such that $0 < h < 1$ and
    \begin{align*}
      h < \frac{x - y^n}{n(y + 1)^{n-1}}.
    \end{align*}
    Let $a = y$, $b = y + h$. Then
    \begin{align*}
      (y + h)^n - y^n < hn(y + h)^{n - 1} < hn(y + 1)^{n - 1} < x - y^n.
    \end{align*}
    Thus $(y + h)^n < x$, and $y + h \in E$. But $y + h > y$, which contradicts the
    fact that $y$ is an upper bound of $E$.

    Now assume $y^n > x$. Let
    \begin{align*}
      k = \frac{y^n - x}{ny^{n-1}};
    \end{align*}
    then $0 < k < y$. If $t \leq y - k$, then
    \begin{align*}
      y^n - t^n \leq y^n - (y - k)^n < kny^{n - 1} = y^n - x.
    \end{align*}
    Therefore $t^n > x$, so $t \notin E$. This implies that $y - k$ is an upper bound
    of $E$. However, $y - k < y$, so this contradicts the fact that $y$ is the least
    upper bound of $E$.

    The only possibility left is that $y^n = x$, which completes the proof.
  \end{proof}
\end{thm}

\begin{cor}
  If $a$ and $b$ are positive real numbers and $n$ is a positive integer, then
  \begin{align*}
    (ab)^{1/n} = a^{1/n}b^{1/n}.
  \end{align*}

  \begin{proof}
    Let $\alpha = a^{1/n}$ and $\beta = b^{1/n}$. Because multiplication in a field
    is commutative, we have
    \begin{align*}
      ab = \alpha^n\beta^n = \alpha \cdots \alpha \cdot \beta \cdots \beta =
      \alpha\beta \cdots \alpha\beta = (\alpha\beta)^n.
    \end{align*}
    By theorem \ref{thm:uniqrealroots}, there is only one real $x$ such that $ab =
    x^n$. Therefore if $ab = (\alpha\beta)^n$,
    \begin{align*}
      (ab)^{1/n} = (\alpha\beta)^{n/n} = \alpha\beta = a^{1/n}b^{1/n}.
    \end{align*}
  \end{proof}
\end{cor}

\begin{comm}
  This is a brief discussion of decimals as they relate to real numbers.

  Let $x > 0$ be real, and let $n_0$ be the largest integer such that $n_0 \leq x$.
  (This is possible by theorem \ref{thm:rarchqdenseinr}.1.) Now choose integers
  $n_1,\cdots,n_{k-1}$, and then let $n_k$ be the largest integer such that
  \begin{align*}
    n_0 + \frac{n_1}{10} + \cdots + \frac{n_k}{10^k} \leq x.
  \end{align*}

  Let $E$ be the set of all such numbers
  \begin{align*}
    n_0 + \frac{n_1}{10} + \cdots + \frac{n_k}{10^k}\ \ (k = 0,1,2,\ldots)
  \end{align*}
  $\leq x$; then $x = \sup E$. The decimal expansion of $x$ is then
  \begin{align*}
    n_0\ .\ n_1n_2n_3\cdots.
  \end{align*}
  Because $E$ is bounded above, this represents the decimal expansion of $\sup E$
  even if it is infinite.
\end{comm}

\begin{exm}
  The field $\mathbb{R}$ is a subfield of $\mathbb{C}$.

  We can represent a real number $x$ as a complex number $(x +
  0i)$. This means that the real numbers $1$ and $0$ are in
  $\mathbb{C}$. It also means that if $x, y$ are real numbers,
  $(x + y)$, $xy$, $-x$, and (if $x \neq 0$) $x^{-1}$ are in
  $\mathbb{C}$.
\end{exm}

\begin{thm}
  Any subfield of $\mathbb{C}$ must contain every rational
  number.
  \begin{proof}
    By contradiction. Assume that $F$ is a subfield of
    $\mathbb{C}$ which omits the rational number $p$, $p \neq 0$.
    We know that for any rational number $q$, there is a rational
    number $r$ such that $qr = p$. This is because $qq^{-1} = 1$,
    and thus $qq^{-1}p = p$; therefore $r = q^{-1}p$. For $F$ to
    be a field, $qr$ would need to produce a result in $F$; since
    $F$ omits $p$, $q$ and $r$ must be omitted as well. But this
    ultimately leaves no rational numbers in $F$ at all, and thus
    $F$ cannot be a field in any sense, let alone a subfield of
    $\mathbb{C}$.
  \end{proof}
\end{thm}

\begin{thm}
  The set of all complex numbers of the form $x + y\sqrt{2}$,
  where $x$ and $y$ are rational, is a subfield of $\mathbb{C}$.

  \begin{proof}
    By lemmas 2.*.
  \end{proof}
\end{thm}

\begin{lemma}
  If $p,q,r,s$ are rational numbers, then $(p + q\sqrt{2}) + (r
  + s\sqrt{2})$ is a complex number of the form $x +
  y\sqrt{2}$ where $x, y$ are rational.
  \begin{proof}
    \begin{align*}
      (p + q\sqrt{2}) + (r + s\sqrt{2}) &=\\
      p + q\sqrt{2} + r + s\sqrt{2} &=\\
      p + r + q\sqrt{2} + s\sqrt{2} &=\\
      (p + r) + (q + s)\sqrt{2}&.
    \end{align*}
    Then $(p + q\sqrt{2}) + (r + s\sqrt{2})$ is a complex number
    of the form $x + y\sqrt{2}$, $x = (p + q)$, $y = (r + s)$.
  \end{proof}
\end{lemma}

\begin{lemma}
  If $p,q,r,s$ are rational numbers, then $(p + q\sqrt{2})
  \cdot (r + s\sqrt{2})$ is a complex number of the form $x +
  y\sqrt{2}$ where $x, y$ are rational.
  \begin{proof}
    \begin{align*}
      (p + q\sqrt{2}) \cdot (r + s\sqrt{2}) &=\\
      pr + qr\sqrt{2} + ps\sqrt{2} + qs(\sqrt{2})^{2} &=\\
      (pr + 2qs) + (qr + ps)\sqrt{2}&.
    \end{align*}
    Then $(p + q\sqrt{2}) \cdot (r + s\sqrt{2})$ is a complex
    number of the form $x + y\sqrt{2}$, $x = (pr + 2qs)$, $y =
    (qr + ps)$.
  \end{proof}
\end{lemma}

\begin{lemma}
  If $p,q$ are rational numbers, then $-(p + q\sqrt{2})$ is a
  complex number of the form $x + y\sqrt{2}$ where $x, y$ are
  rational.
  \begin{proof}
    $-(p + q\sqrt{2}) = -p + (-q)\sqrt{2}$. Then $-(p +
    q\sqrt{2})$ is a complex number of the form $x + y\sqrt{2}$,
    $x = -p$, $y = -q$.
  \end{proof}
\end{lemma}

\begin{lemma}
  If $p,q$ are rational numbers and $p + q\sqrt{2} \neq 0$, then
  $(p + q\sqrt{2})^{-1}$ is a complex number of the form $x +
  y\sqrt{2}$ where $x, y$ are rational.
  \begin{proof}
    \begin{align*}
      (p + q\sqrt{2})^{-1} &=\\
      \frac{1}{p + q\sqrt{2}} &=\\
      \frac{p - q\sqrt{2}}{(p + q\sqrt{2})(p - q\sqrt{2})} &=\\
      \frac{p - q\sqrt{2}}{p^{2} - 2q^{2}} &=\\
      \frac{p}{p^{2} - 2q^{2}} - \frac{q}{p^{2} - 2q^{2}}\sqrt{2}&.
    \end{align*}
    Then $(p + q\sqrt{2})^{-1}$ is a complex number of the form
    $x + y\sqrt{2}$, $x = \frac{p}{p^{2} - 2q^{2}}$, $y =
    -\frac{q}{p^{2} - 2q^{2}}$.
  \end{proof}
\end{lemma}

\begin{defn}
  A \textbf{scalar} is an element of a field.
\end{defn}

\begin{comm}
  If $x, y$ are scalars from a subfield $F$ of $\mathbb{C}$, then
  the performance of addition, multiplication, subtraction, or
  division with $x$ and $y$ does not leave $F$.
\end{comm}

\begin{comm}
  In some fields, it is possible to add $1$ to itself a finite
  number of times and obtain $0$, i.e.
  \begin{center}
    $1 + 1 + … + 1 = 0.$
  \end{center}
  However, this is not the case for $\mathbb{C}$, nor any
  subfield of it.
\end{comm}

\begin{defn}
  If a field $F$ has the property that it is possible to add $1$
  to itself a finite number of times and obtain $0$ in it, the
  least $n$ such that the sum of $n$ $1$s yields $0$ is called
  the \textbf{characteristic} of $F$. If $F$ does not have this
  property, it is said to be of \textbf{characteristic zero}.
\end{defn}

\begin{comm}
  Often, when assuming that $F$ is a subfield of $\mathbb{C}$,
  what is desired is to ensure that $F$ is a field of
  characteristic zero.
\end{comm}

\end{document}
